Json wip

typeclass/Json1.fst
@@ -183,7 +183,8 @@ val testb : #st_a:Type0 -> #st_b:Type0 -> #o_a:eqtype -> #o_b:eqtype -> #m:(json
         [SMTPat (m.eq_b a b)]
 let testb #st_a #st_b #o_a #o_b #m a b = 
   m.lem_eq_b a b
-  
+
+#set-options "--z3rlimit 300 --ifuel 3"
 class vc (st_a st_b:Type0) (o_a o_b:eqtype) (m:json st_a st_b o_a o_b) = {
  merge_comm_a : l:st_a -> a:st_a -> b:st_a ->
   Lemma (ensures m.eq_a (m.merge_a l a b) (m.merge_a l b a));
@@ -219,6 +220,128 @@ class vc (st_a st_b:Type0) (o_a o_b:eqtype) (m:json st_a st_b o_a o_b) = {
           (ensures eq (merge (init_st t) (do (init_st t) o1) (do (init_st t) o2)) 
                       (do #st_a #st_b #o_a #o_b #m (merge (init_st t) (init_st t) (do (init_st t) o2)) o1));
 
+ ind_lca_2op_a : l:st_a -> o1:op_a -> o2:op_a -> ol:op_a ->
+   Lemma (requires (Fst_then_snd? (rc_a #st_a #st_b #o_a #o_b #m o2 o1) \/ Either? (rc_a #st_a #st_b #o_a #o_b #m o2 o1)) /\ get_rid o1 <> get_rid o2 /\
+                    distinct_ops o1 o2 /\ distinct_ops o1 ol /\ distinct_ops o2 ol /\
+                    m.eq_a (m.merge_a l (m.do_a l o1) (m.do_a l o2)) (m.do_a (m.merge_a l l (m.do_a l o2)) o1))
+         (ensures m.eq_a (m.merge_a (m.do_a l ol) (m.do_a (m.do_a l ol) o1) (m.do_a (m.do_a l ol) o2)) (m.do_a (m.merge_a (m.do_a l ol) (m.do_a l ol) (m.do_a (m.do_a l ol) o2)) o1));
+
+ ind_lca_2op_b : l:st_b -> o1:op_b -> o2:op_b -> ol:op_b ->
+   Lemma (requires (Fst_then_snd? (m.rc_b o2 o1) \/ Either? (m.rc_b o2 o1)) /\ get_rid o1 <> get_rid o2 /\
+                    distinct_ops o1 o2 /\ distinct_ops o1 ol /\ distinct_ops o2 ol /\
+                    m.eq_b (m.merge_b l (m.do_b l o1) (m.do_b l o2)) (m.do_b (m.merge_b l l (m.do_b l o2)) o1))
+         (ensures m.eq_b (m.merge_b (m.do_b l ol) (m.do_b (m.do_b l ol) o1) (m.do_b (m.do_b l ol) o2)) (m.do_b (m.merge_b (m.do_b l ol) (m.do_b l ol) (m.do_b (m.do_b l ol) o2)) o1));
+
+ ind_lca_2op' : l:st -> o1:op -> o2:op -> ol:op ->
+   Lemma (requires Either? (rc #st_a #st_b #o_a #o_b #m o2 o1) /\ get_rid o1 <> get_rid o2 /\
+                    distinct_ops o1 o2 /\ distinct_ops o1 ol /\ distinct_ops o2 ol /\
+                    ~ (get_key o1 = get_key ol && get_key o2 = get_key ol /\
+                       is_alpha_op o1 /\ is_alpha_op o2 /\ is_alpha_op ol /\ (Fst_then_snd? (m.rc_a (get_op_a o2) (get_op_a o1)) || Either? (m.rc_a (get_op_a o2) (get_op_a o1))) /\
+                       is_beta_op o1 /\ is_beta_op o2 /\ is_beta_op ol /\ (Fst_then_snd? (m.rc_b (get_op_b o2) (get_op_b o1)) || Either? (m.rc_b (get_op_b o2) (get_op_b o1)))) /\
+                    eq (merge l (do l o1) (do l o2)) (do (merge l l (do l o2)) o1))
+          (ensures eq (merge (do #st_a #st_b #o_a #o_b #m l ol) (do (do l ol) o1) (do (do l ol) o2)) (do (merge (do l ol) (do l ol) (do (do l ol) o2)) o1));
+
+ inter_right_base_2op_a : l:st_a -> a:st_a -> b:st_a -> o1:op_a -> o2:op_a -> ob:op_a -> ol:op_a ->
+   Lemma (requires (Fst_then_snd? (m.rc_a o2 o1) \/ Either? (m.rc_a o2 o1)) /\ get_rid o1 <> get_rid o2 /\ Fst_then_snd? (m.rc_a ob ol) /\ get_rid ob <> get_rid ol /\
+                    distinct_ops o1 o2 /\ distinct_ops o1 ob /\ distinct_ops o1 ol /\ distinct_ops o2 ob /\ distinct_ops o2 ol /\ distinct_ops ob ol /\
+                    m.eq_a (m.merge_a l (m.do_a a o1) (m.do_a b o2)) (m.do_a (m.merge_a l a (m.do_a b o2)) o1) /\ //from pre-cond of ind_right_2op
+                    m.eq_a (m.merge_a l (m.do_a a o1) (m.do_a (m.do_a b ob) o2)) (m.do_a (m.merge_a l a (m.do_a (m.do_a b ob) o2)) o1) /\ //from ind_right_2op
+                    m.eq_a (m.merge_a (m.do_a l ol) (m.do_a (m.do_a a ol) o1) (m.do_a (m.do_a b ol) o2)) (m.do_a (m.merge_a (m.do_a l ol) (m.do_a a ol) (m.do_a (m.do_a b ol) o2)) o1))
+         (ensures m.eq_a (m.merge_a (m.do_a l ol) (m.do_a (m.do_a a ol) o1) (m.do_a (m.do_a (m.do_a b ob) ol) o2)) (m.do_a (m.merge_a (m.do_a l ol) (m.do_a a ol) (m.do_a (m.do_a (m.do_a b ob) ol) o2)) o1));
+
+ inter_right_base_2op_b : l:st_b -> a:st_b -> b:st_b -> o1:op_b -> o2:op_b -> ob:op_b -> ol:op_b ->
+   Lemma (requires (Fst_then_snd? (m.rc_b o2 o1) \/ Either? (m.rc_b o2 o1)) /\ get_rid o1 <> get_rid o2 /\ Fst_then_snd? (m.rc_b ob ol) /\ get_rid ob <> get_rid ol /\
+                    distinct_ops o1 o2 /\ distinct_ops o1 ob /\ distinct_ops o1 ol /\ distinct_ops o2 ob /\ distinct_ops o2 ol /\ distinct_ops ob ol /\
+                    m.eq_b (m.merge_b l (m.do_b a o1) (m.do_b b o2)) (m.do_b (m.merge_b l a (m.do_b b o2)) o1) /\ //from pre-cond of ind_right_2op
+                    m.eq_b (m.merge_b l (m.do_b a o1) (m.do_b (m.do_b b ob) o2)) (m.do_b (m.merge_b l a (m.do_b (m.do_b b ob) o2)) o1) /\ //from ind_right_2op
+                    m.eq_b (m.merge_b (m.do_b l ol) (m.do_b (m.do_b a ol) o1) (m.do_b (m.do_b b ol) o2)) (m.do_b (m.merge_b (m.do_b l ol) (m.do_b a ol) (m.do_b (m.do_b b ol) o2)) o1))
+         (ensures m.eq_b (m.merge_b (m.do_b l ol) (m.do_b (m.do_b a ol) o1) (m.do_b (m.do_b (m.do_b b ob) ol) o2)) (m.do_b (m.merge_b (m.do_b l ol) (m.do_b a ol) (m.do_b (m.do_b (m.do_b b ob) ol) o2)) o1));
+          
+ inter_right_base_2op' : l:st -> a:st -> b:st -> o1:op -> o2:op -> ob:op -> ol:op ->
+   Lemma (requires Either? (rc #st_a #st_b #o_a #o_b #m o2 o1) /\ get_rid o1 <> get_rid o2 /\ Fst_then_snd? (rc #st_a #st_b #o_a #o_b #m ob ol) /\ get_rid ob <> get_rid ol /\
+                    distinct_ops o1 o2 /\ distinct_ops o1 ob /\ distinct_ops o1 ol /\ distinct_ops o2 ob /\ distinct_ops o2 ol /\ distinct_ops ob ol /\
+                    ~ (get_key o1 = get_key ol && get_key o2 = get_key ol /\ get_key ob = get_key ol /\
+                       is_alpha_op o1 /\ is_alpha_op o2 /\ is_alpha_op ob /\ is_alpha_op ol /\ (Fst_then_snd? (m.rc_a (get_op_a o2) (get_op_a o1)) || Either? (m.rc_a (get_op_a o2) (get_op_a o1))) /\ Fst_then_snd? (m.rc_a (get_op_a ob) (get_op_a ol)) /\
+                       is_beta_op o1 /\ is_beta_op o2 /\ is_beta_op ob /\ is_beta_op ol /\ (Fst_then_snd? (m.rc_b (get_op_b o2) (get_op_b o1)) || Either? (m.rc_b (get_op_b o2) (get_op_b o1))) /\ Fst_then_snd? (m.rc_b (get_op_b ob) (get_op_b ol))) /\
+                    eq (merge l (do a o1) (do b o2)) (do (merge l a (do b o2)) o1) /\ //from pre-cond of ind_right_2op
+                    eq (merge l (do a o1) (do (do b ob) o2)) (do (merge l a (do (do b ob) o2)) o1) /\ //from ind_right_2op
+                    eq (merge (do l ol) (do (do a ol) o1) (do (do b ol) o2)) (do (merge (do l ol) (do a ol) (do (do b ol) o2)) o1))
+         (ensures eq (merge (do l ol) (do (do a ol) o1) (do (do (do b ob) ol) o2)) (do (merge (do #st_a #st_b #o_a #o_b #m l ol) (do a ol) (do (do (do b ob) ol) o2)) o1));
+
+  inter_left_base_2op_a : l:st_a -> a:st_a -> b:st_a -> o1:op_a -> o2:op_a -> ob:op_a -> ol:op_a ->
+   Lemma (requires (Fst_then_snd? (m.rc_a o2 o1) \/ Either? (m.rc_a o2 o1)) /\ get_rid o1 <> get_rid o2 /\ Fst_then_snd? (m.rc_a ob ol) /\ get_rid ob <> get_rid ol /\
+                    distinct_ops o1 o2 /\ distinct_ops o1 ob /\ distinct_ops o1 ol /\ distinct_ops o2 ob /\ distinct_ops o2 ol /\ distinct_ops ob ol /\
+                    m.eq_a (m.merge_a (m.do_a l ol) (m.do_a (m.do_a a ol) o1) (m.do_a (m.do_a b ol) o2)) (m.do_a (m.merge_a (m.do_a l ol) (m.do_a a ol) (m.do_a (m.do_a b ol) o2)) o1))
+         (ensures m.eq_a (m.merge_a (m.do_a l ol) (m.do_a (m.do_a (m.do_a a ob) ol) o1) (m.do_a (m.do_a b ol) o2)) (m.do_a (m.merge_a (m.do_a l ol) (m.do_a (m.do_a a ob) ol) (m.do_a (m.do_a b ol) o2)) o1));
+
+ inter_left_base_2op_b : l:st_b -> a:st_b -> b:st_b -> o1:op_b -> o2:op_b -> ob:op_b -> ol:op_b ->
+   Lemma (requires (Fst_then_snd? (m.rc_b o2 o1) \/ Either? (m.rc_b o2 o1)) /\ get_rid o1 <> get_rid o2 /\ Fst_then_snd? (m.rc_b ob ol) /\ get_rid ob <> get_rid ol /\
+                    distinct_ops o1 o2 /\ distinct_ops o1 ob /\ distinct_ops o1 ol /\ distinct_ops o2 ob /\ distinct_ops o2 ol /\ distinct_ops ob ol /\
+                    m.eq_b (m.merge_b (m.do_b l ol) (m.do_b (m.do_b a ol) o1) (m.do_b (m.do_b b ol) o2)) (m.do_b (m.merge_b (m.do_b l ol) (m.do_b a ol) (m.do_b (m.do_b b ol) o2)) o1))
+         (ensures m.eq_b (m.merge_b (m.do_b l ol) (m.do_b (m.do_b (m.do_b a ob) ol) o1) (m.do_b (m.do_b b ol) o2)) (m.do_b (m.merge_b (m.do_b l ol) (m.do_b (m.do_b a ob) ol) (m.do_b (m.do_b b ol) o2)) o1));
+          
+ inter_left_base_2op' : l:st -> a:st -> b:st -> o1:op -> o2:op -> ob:op -> ol:op ->
+   Lemma (requires Either? (rc #st_a #st_b #o_a #o_b #m o2 o1) /\ get_rid o1 <> get_rid o2 /\ Fst_then_snd? (rc #st_a #st_b #o_a #o_b #m ob ol) /\ get_rid ob <> get_rid ol /\
+                    distinct_ops o1 o2 /\ distinct_ops o1 ob /\ distinct_ops o1 ol /\ distinct_ops o2 ob /\ distinct_ops o2 ol /\ distinct_ops ob ol /\
+                    ~ (get_key o1 = get_key ol && get_key o2 = get_key ol /\ get_key ob = get_key ol /\
+                       is_alpha_op o1 /\ is_alpha_op o2 /\ is_alpha_op ob /\ is_alpha_op ol /\ (Fst_then_snd? (m.rc_a (get_op_a o2) (get_op_a o1)) || Either? (m.rc_a (get_op_a o2) (get_op_a o1))) /\ Fst_then_snd? (m.rc_a (get_op_a ob) (get_op_a ol)) /\
+                       is_beta_op o1 /\ is_beta_op o2 /\ is_beta_op ob /\ is_beta_op ol /\ (Fst_then_snd? (m.rc_b (get_op_b o2) (get_op_b o1)) || Either? (m.rc_b (get_op_b o2) (get_op_b o1))) /\ Fst_then_snd? (m.rc_b (get_op_b ob) (get_op_b ol))) /\
+                    eq (merge (do l ol) (do (do a ol) o1) (do (do b ol) o2)) (do (merge (do l ol) (do a ol) (do (do b ol) o2)) o1))
+         (ensures eq (merge (do l ol) (do (do (do a ob) ol) o1) (do (do b ol) o2)) (do (merge (do #st_a #st_b #o_a #o_b #m l ol) (do (do a ob) ol) (do (do b ol) o2)) o1));
+
+ inter_right_2op_a : l:st_a -> a:st_a -> b:st_a -> o1:op_a -> o2:op_a -> ob:op_a -> ol:op_a -> o:op_a ->
+   Lemma (requires (Fst_then_snd? (m.rc_a o2 o1) \/ Either? (m.rc_a o2 o1)) /\ get_rid o1 <> get_rid o2 /\ Fst_then_snd? (m.rc_a ob ol) /\ get_rid ob <> get_rid ol /\
+                    (~ (Either? (m.rc_a o ob)) \/ Fst_then_snd? (m.rc_a o ol)) /\
+                    distinct_ops o1 o2 /\ distinct_ops o1 ob /\ distinct_ops o1 ol /\ distinct_ops o1 o /\ distinct_ops o2 ob /\ distinct_ops o2 ol /\ distinct_ops o2 o /\ distinct_ops ob ol /\ distinct_ops ob o /\ distinct_ops ol o /\
+                    get_rid o <> get_rid ol /\
+                    m.eq_a (m.merge_a (m.do_a l ol) (m.do_a (m.do_a a ol) o1) (m.do_a (m.do_a (m.do_a b ob) ol) o2)) (m.do_a (m.merge_a (m.do_a l ol) (m.do_a a ol) (m.do_a (m.do_a (m.do_a b ob) ol) o2)) o1))
+         (ensures m.eq_a (m.merge_a (m.do_a l ol) (m.do_a (m.do_a a ol) o1) (m.do_a (m.do_a (m.do_a (m.do_a b o) ob) ol) o2)) (m.do_a (m.merge_a (m.do_a l ol) (m.do_a a ol) (m.do_a (m.do_a (m.do_a (m.do_a b o) ob) ol) o2)) o1));
+
+ inter_right_2op_b : l:st_b -> a:st_b -> b:st_b -> o1:op_b -> o2:op_b -> ob:op_b -> ol:op_b -> o:op_b ->
+   Lemma (requires (Fst_then_snd? (m.rc_b o2 o1) \/ Either? (m.rc_b o2 o1)) /\ get_rid o1 <> get_rid o2 /\ Fst_then_snd? (m.rc_b ob ol) /\ get_rid ob <> get_rid ol /\
+                    (~ (Either? (m.rc_b o ob)) \/ Fst_then_snd? (m.rc_b o ol)) /\
+                    distinct_ops o1 o2 /\ distinct_ops o1 ob /\ distinct_ops o1 ol /\ distinct_ops o1 o /\ distinct_ops o2 ob /\ distinct_ops o2 ol /\ distinct_ops o2 o /\ distinct_ops ob ol /\ distinct_ops ob o /\ distinct_ops ol o /\
+                    get_rid o <> get_rid ol /\
+                    m.eq_b (m.merge_b (m.do_b l ol) (m.do_b (m.do_b a ol) o1) (m.do_b (m.do_b (m.do_b b ob) ol) o2)) (m.do_b (m.merge_b (m.do_b l ol) (m.do_b a ol) (m.do_b (m.do_b (m.do_b b ob) ol) o2)) o1))
+         (ensures m.eq_b (m.merge_b (m.do_b l ol) (m.do_b (m.do_b a ol) o1) (m.do_b (m.do_b (m.do_b (m.do_b b o) ob) ol) o2)) (m.do_b (m.merge_b (m.do_b l ol) (m.do_b a ol) (m.do_b (m.do_b (m.do_b (m.do_b b o) ob) ol) o2)) o1));
+          
+  inter_right_2op' : l:st -> a:st -> b:st -> o1:op -> o2:op -> ob:op -> ol:op -> o:op ->
+    Lemma (requires Either? (rc #st_a #st_b #o_a #o_b #m o2 o1) /\ get_rid o1 <> get_rid o2 /\ Fst_then_snd? (rc #st_a #st_b #o_a #o_b #m ob ol) /\ get_rid ob <> get_rid ol /\
+                    (~ (Either? (rc #st_a #st_b #o_a #o_b #m o ob)) \/ Fst_then_snd? (rc #st_a #st_b #o_a #o_b #m o ol)) /\
+                    distinct_ops o1 o2 /\ distinct_ops o1 ob /\ distinct_ops o1 ol /\ distinct_ops o1 o /\ distinct_ops o2 ob /\ distinct_ops o2 ol /\ distinct_ops o2 o /\ distinct_ops ob ol /\ distinct_ops ob o /\ distinct_ops ol o /\
+                    get_rid o <> get_rid ol /\
+                    ~ (get_key o1 = get_key o && get_key o2 = get_key o /\ get_key ob = get_key o /\ get_key ol = get_key o /\
+                       is_alpha_op o1 /\ is_alpha_op o2 /\ is_alpha_op ob /\ is_alpha_op ol /\ is_alpha_op o /\ (Fst_then_snd? (m.rc_a (get_op_a o2) (get_op_a o1)) \/ Either? (m.rc_a (get_op_a o2) (get_op_a o1))) /\ Fst_then_snd? (m.rc_a (get_op_a ob) (get_op_a ol)) /\ (Fst_then_snd? (m.rc_a (get_op_a o) (get_op_a ob)) \/ Snd_then_fst? (m.rc_a (get_op_a o) (get_op_a ob)) \/ Fst_then_snd? (m.rc_a (get_op_a o) (get_op_a ol))) /\
+                       is_beta_op o1 /\ is_beta_op o2 /\ is_beta_op ob /\ is_beta_op ol /\ is_beta_op o /\ (Fst_then_snd? (m.rc_b (get_op_b o2) (get_op_b o1)) \/ Either? (m.rc_b (get_op_b o2) (get_op_b o1))) /\ Fst_then_snd? (m.rc_b (get_op_b ob) (get_op_b ol)) /\ (Fst_then_snd? (m.rc_b (get_op_b o) (get_op_b ob)) \/ Snd_then_fst? (m.rc_b (get_op_b o) (get_op_b ob)) \/ Fst_then_snd? (m.rc_b (get_op_b o) (get_op_b ol)))) /\
+                    eq (merge (do l ol) (do (do a ol) o1) (do (do (do b ob) ol) o2)) (do (merge (do l ol) (do a ol) (do (do (do b ob) ol) o2)) o1))
+         (ensures eq (merge (do l ol) (do (do a ol) o1) (do (do (do (do b o) ob) ol) o2)) (do (merge (do #st_a #st_b #o_a #o_b #m l ol) (do a ol) (do (do (do (do b o) ob) ol) o2)) o1));
+
+ inter_left_2op_a : l:st_a -> a:st_a -> b:st_a -> o1:op_a -> o2:op_a -> ob:op_a -> ol:op_a -> o:op_a ->
+   Lemma (requires (Fst_then_snd? (m.rc_a o2 o1) \/ Either? (m.rc_a o2 o1)) /\ get_rid o1 <> get_rid o2 /\ Fst_then_snd? (m.rc_a ob ol) /\ get_rid ob <> get_rid ol /\
+                    (~ (Either? (m.rc_a o ob)) \/ Fst_then_snd? (m.rc_a o ol)) /\
+                    distinct_ops o1 o2 /\ distinct_ops o1 ob /\ distinct_ops o1 ol /\ distinct_ops o1 o /\ distinct_ops o2 ob /\ distinct_ops o2 ol /\ distinct_ops o2 o /\ distinct_ops ob ol /\ distinct_ops ob o /\ distinct_ops ol o /\
+                    get_rid o <> get_rid ol /\
+                    m.eq_a (m.merge_a (m.do_a l ol) (m.do_a (m.do_a a ol) o1) (m.do_a (m.do_a (m.do_a b ob) ol) o2)) (m.do_a (m.merge_a (m.do_a l ol) (m.do_a a ol) (m.do_a (m.do_a (m.do_a b ob) ol) o2)) o1))
+          (ensures m.eq_a (m.merge_a (m.do_a l ol) (m.do_a (m.do_a (m.do_a a o) ol) o1) (m.do_a (m.do_a (m.do_a b ob) ol) o2)) (m.do_a (m.merge_a (m.do_a l ol) (m.do_a (m.do_a a o) ol) (m.do_a (m.do_a (m.do_a b ob) ol) o2)) o1));
+
+ inter_left_2op_b : l:st_b -> a:st_b -> b:st_b -> o1:op_b -> o2:op_b -> ob:op_b -> ol:op_b -> o:op_b ->
+   Lemma (requires (Fst_then_snd? (m.rc_b o2 o1) \/ Either? (m.rc_b o2 o1)) /\ get_rid o1 <> get_rid o2 /\ Fst_then_snd? (m.rc_b ob ol) /\ get_rid ob <> get_rid ol /\
+                    (~ (Either? (m.rc_b o ob)) \/ Fst_then_snd? (m.rc_b o ol)) /\
+                    distinct_ops o1 o2 /\ distinct_ops o1 ob /\ distinct_ops o1 ol /\ distinct_ops o1 o /\ distinct_ops o2 ob /\ distinct_ops o2 ol /\ distinct_ops o2 o /\ distinct_ops ob ol /\ distinct_ops ob o /\ distinct_ops ol o /\
+                    get_rid o <> get_rid ol /\
+                    m.eq_b (m.merge_b (m.do_b l ol) (m.do_b (m.do_b a ol) o1) (m.do_b (m.do_b (m.do_b b ob) ol) o2)) (m.do_b (m.merge_b (m.do_b l ol) (m.do_b a ol) (m.do_b (m.do_b (m.do_b b ob) ol) o2)) o1))
+         (ensures m.eq_b (m.merge_b (m.do_b l ol) (m.do_b (m.do_b (m.do_b a o) ol) o1) (m.do_b (m.do_b (m.do_b b ob) ol) o2)) (m.do_b (m.merge_b (m.do_b l ol) (m.do_b (m.do_b a o) ol) (m.do_b (m.do_b (m.do_b b ob) ol) o2)) o1));
+          
+ inter_left_2op' : l:st -> a:st -> b:st -> o1:op -> o2:op -> ob:op -> ol:op -> o:op ->
+   Lemma (requires Either? (rc #st_a #st_b #o_a #o_b #m o2 o1) /\ get_rid o1 <> get_rid o2 /\ Fst_then_snd? (rc #st_a #st_b #o_a #o_b #m ob ol) /\ get_rid ob <> get_rid ol /\
+                    distinct_ops o1 o2 /\ distinct_ops o1 ob /\ distinct_ops o1 ol /\ distinct_ops o1 o /\ distinct_ops o2 ob /\ distinct_ops o2 ol /\ distinct_ops o2 o /\ distinct_ops ob ol /\ distinct_ops ob o /\ distinct_ops ol o /\
+                    get_rid o <> get_rid ol /\
+                    ~ (get_key o1 = get_key o && get_key o2 = get_key o /\ get_key ob = get_key o /\ get_key ol = get_key o /\
+                       is_alpha_op o1 /\ is_alpha_op o2 /\ is_alpha_op ob /\ is_alpha_op ol /\ is_alpha_op o /\ (Fst_then_snd? (m.rc_a (get_op_a o2) (get_op_a o1)) \/ Either? (m.rc_a (get_op_a o2) (get_op_a o1))) /\ Fst_then_snd? (m.rc_a (get_op_a ob) (get_op_a ol)) /\ (Fst_then_snd? (m.rc_a (get_op_a o) (get_op_a ob)) \/ Snd_then_fst? (m.rc_a (get_op_a o) (get_op_a ob)) \/ Fst_then_snd? (m.rc_a (get_op_a o) (get_op_a ol))) /\
+                       is_beta_op o1 /\ is_beta_op o2 /\ is_beta_op ob /\ is_beta_op ol /\ is_beta_op o /\ (Fst_then_snd? (m.rc_b (get_op_b o2) (get_op_b o1)) \/ Either? (m.rc_b (get_op_b o2) (get_op_b o1))) /\ Fst_then_snd? (m.rc_b (get_op_b ob) (get_op_b ol)) /\ (Fst_then_snd? (m.rc_b (get_op_b o) (get_op_b ob)) \/ Snd_then_fst? (m.rc_b (get_op_b o) (get_op_b ob)) \/ Fst_then_snd? (m.rc_b (get_op_b o) (get_op_b ol)))) /\
+                    eq (merge (do l ol) (do (do a ol) o1) (do (do (do b ob) ol) o2)) (do (merge (do l ol) (do a ol) (do (do (do b ob) ol) o2)) o1))
+         (ensures eq (merge (do l ol) (do (do (do a o) ol) o1) (do (do (do b ob) ol) o2)) (do (merge (do #st_a #st_b #o_a #o_b #m l ol) (do (do a o) ol) (do (do (do b ob) ol) o2)) o1));
+          
  ind_right_2op_a : l:st_a -> a:st_a -> b:st_a -> o1:op_a -> o2:op_a -> o2':op_a ->
   Lemma (requires Fst_then_snd? (m.rc_a o2 o1) /\ get_rid o1 <> get_rid o2 /\
                     distinct_ops o1 o2 /\ distinct_ops o1 o2' /\ distinct_ops o2 o2' /\
@@ -229,10 +352,21 @@ class vc (st_a st_b:Type0) (o_a o_b:eqtype) (m:json st_a st_b o_a o_b) = {
    Lemma (requires Fst_then_snd? (m.rc_b o2 o1) /\ get_rid o1 <> get_rid o2 /\
                     distinct_ops o1 o2 /\ distinct_ops o1 o2' /\ distinct_ops o2 o2' /\
                     m.eq_b (m.merge_b l (m.do_b a o1) (m.do_b b o2)) (m.do_b (m.merge_b l a (m.do_b b o2)) o1))
-         (ensures m.eq_b (m.merge_b l (m.do_b a o1) (m.do_b (m.do_b b o2') o2)) (m.do_b (m.merge_b l a (m.do_b (m.do_b b o2') o2)) o1))
+         (ensures m.eq_b (m.merge_b l (m.do_b a o1) (m.do_b (m.do_b b o2') o2)) (m.do_b (m.merge_b l a (m.do_b (m.do_b b o2') o2)) o1));
+
+ ind_left_2op_a : l:st_a -> a:st_a -> b:st_a -> o1:op_a -> o2:op_a -> o1':op_a ->
+   Lemma (requires Fst_then_snd? (m.rc_a o2 o1) /\ get_rid o1 <> get_rid o2 /\
+                    distinct_ops o1 o2 /\ distinct_ops o1 o1' /\ distinct_ops o2 o1' /\
+                    m.eq_a (m.merge_a l (m.do_a a o1) (m.do_a b o2)) (m.do_a (m.merge_a l a (m.do_a b o2)) o1))
+         (ensures m.eq_a (m.merge_a l (m.do_a (m.do_a a o1') o1) (m.do_a b o2)) (m.do_a (m.merge_a l (m.do_a a o1') (m.do_a b o2)) o1));
+
+ ind_left_2op_b : l:st_b -> a:st_b -> b:st_b -> o1:op_b -> o2:op_b -> o1':op_b ->
+   Lemma (requires Fst_then_snd? (m.rc_b o2 o1) /\ get_rid o1 <> get_rid o2 /\
+                    distinct_ops o1 o2 /\ distinct_ops o1 o1' /\ distinct_ops o2 o1' /\
+                    m.eq_b (m.merge_b l (m.do_b a o1) (m.do_b b o2)) (m.do_b (m.merge_b l a (m.do_b b o2)) o1))
+         (ensures m.eq_b (m.merge_b l (m.do_b (m.do_b a o1') o1) (m.do_b b o2)) (m.do_b (m.merge_b l (m.do_b a o1') (m.do_b b o2)) o1))
 }
 
-#set-options "--z3rlimit 100 --ifuel 3"
 val comma : #st_a:Type0 -> #st_b:Type0 -> #o_a:eqtype -> #o_b:eqtype -> #m:(json st_a st_b o_a o_b) -> #v:(vc st_a st_b o_a o_b m) -> l:st_a -> a:st_a -> b:st_a ->
   Lemma (ensures (m.eq_a (m.merge_a l a b) (m.merge_a l b a))) 
         [SMTPat (m.merge_a l a b)]        
@@ -280,6 +414,92 @@ let base_2op #st_a #st_b #o_a #o_b #m #v o1 o2 t =
   else if Either? (rc #st_a #st_b #o_a #o_b #m o2 o1) then v.base_2op' o1 o2 t
   else ()
 
+val ind_lca_2op : #st_a:Type0 -> #st_b:Type0 -> #o_a:eqtype -> #o_b:eqtype -> #m:(json st_a st_b o_a o_b) -> #v:(vc st_a st_b o_a o_b m) -> l:st #st_a #st_b #o_a #o_b #m -> o1:op -> o2:op -> ol:op ->
+  Lemma (requires (Fst_then_snd? (rc #st_a #st_b #o_a #o_b #m o2 o1) \/ Either? (rc #st_a #st_b #o_a #o_b #m o2 o1)) /\ get_rid o1 <> get_rid o2 /\
+                    distinct_ops o1 o2 /\ distinct_ops o1 ol /\ distinct_ops o2 ol /\
+                    eq (merge l (do l o1) (do l o2)) (do (merge l l (do l o2)) o1))
+          (ensures eq (merge (do l ol) (do (do l ol) o1) (do (do l ol) o2)) (do (merge (do l ol) (do l ol) (do (do l ol) o2)) o1))
+          
+let ind_lca_2op #st_a #st_b #o_a #o_b #m #v l o1 o2 ol =
+  let k = get_key ol in
+  let ka = Alpha_t k in let kb = Beta_t k in
+  if get_key o1 = k && get_key o2 = k && is_alpha_op o1 && is_alpha_op o2 && is_alpha_op ol && (Fst_then_snd? (m.rc_a (get_op_a o2) (get_op_a o1)) || Either? (m.rc_a (get_op_a o2) (get_op_a o1))) then
+      v.ind_lca_2op_a (sel l ka) (get_op_a o1) (get_op_a o2) (get_op_a ol)
+  else if get_key o1 = k && get_key o2 = k && is_beta_op o1 && is_beta_op o2 && is_beta_op ol && (Fst_then_snd? (m.rc_b (get_op_b o2) (get_op_b o1)) || Either? (m.rc_b (get_op_b o2) (get_op_b o1))) then
+      v.ind_lca_2op_b (sel l kb) (get_op_b o1) (get_op_b o2) (get_op_b ol)
+  else if Either? (rc #st_a #st_b #o_a #o_b #m o2 o1) then v.ind_lca_2op' l o1 o2 ol
+  else ()
+
+val inter_right_base_2op : #st_a:Type0 -> #st_b:Type0 -> #o_a:eqtype -> #o_b:eqtype -> #m:(json st_a st_b o_a o_b) -> #v:(vc st_a st_b o_a o_b m) -> l:st #st_a #st_b #o_a #o_b #m -> a:st -> b:st -> o1:op -> o2:op -> ob:op -> ol:op ->
+  Lemma (requires (Fst_then_snd? (rc #st_a #st_b #o_a #o_b #m o2 o1) \/ Either? (rc #st_a #st_b #o_a #o_b #m o2 o1)) /\ get_rid o1 <> get_rid o2 /\ Fst_then_snd? (rc #st_a #st_b #o_a #o_b #m ob ol) /\ get_rid ob <> get_rid ol /\
+                    distinct_ops o1 o2 /\ distinct_ops o1 ob /\ distinct_ops o1 ol /\ distinct_ops o2 ob /\ distinct_ops o2 ol /\ distinct_ops ob ol /\
+                    eq (merge l (do a o1) (do b o2)) (do (merge l a (do b o2)) o1) /\ //from pre-cond of ind_right_2op
+                    eq (merge l (do a o1) (do (do b ob) o2)) (do (merge l a (do (do b ob) o2)) o1) /\ //from ind_right_2op
+                    eq (merge (do l ol) (do (do a ol) o1) (do (do b ol) o2)) (do (merge (do l ol) (do a ol) (do (do b ol) o2)) o1))
+          (ensures eq (merge (do l ol) (do (do a ol) o1) (do (do (do b ob) ol) o2)) (do (merge (do l ol) (do a ol) (do (do (do b ob) ol) o2)) o1))
+          
+let inter_right_base_2op #st_a #st_b #o_a #o_b #m #v l a b o1 o2 ob ol =
+  let k = get_key ol in
+  let ka = Alpha_t k in let kb = Beta_t k in
+  if get_key o1 = k && get_key o2 = k && get_key ob = k && is_alpha_op o1 && is_alpha_op o2 && is_alpha_op ob && is_alpha_op ol && (Fst_then_snd? (m.rc_a (get_op_a o2) (get_op_a o1)) || Either? (m.rc_a (get_op_a o2) (get_op_a o1))) && Fst_then_snd? (m.rc_a (get_op_a ob) (get_op_a ol)) then
+      v.inter_right_base_2op_a (sel l ka) (sel a ka) (sel b ka) (get_op_a o1) (get_op_a o2) (get_op_a ob) (get_op_a ol)
+  else if get_key o1 = k && get_key o2 = k && get_key ob = k && is_beta_op o1 && is_beta_op o2 && is_beta_op ob && is_beta_op ol && (Fst_then_snd? (m.rc_b (get_op_b o2) (get_op_b o1)) || Either? (m.rc_b (get_op_b o2) (get_op_b o1))) && Fst_then_snd? (m.rc_b (get_op_b ob) (get_op_b ol)) then
+      v.inter_right_base_2op_b (sel l kb) (sel a kb) (sel b kb) (get_op_b o1) (get_op_b o2) (get_op_b ob) (get_op_b ol)
+  else if Either? (rc #st_a #st_b #o_a #o_b #m o2 o1) then v.inter_right_base_2op' l a b o1 o2 ob ol
+  else ()
+
+val inter_left_base_2op : #st_a:Type0 -> #st_b:Type0 -> #o_a:eqtype -> #o_b:eqtype -> #m:(json st_a st_b o_a o_b) -> #v:(vc st_a st_b o_a o_b m) -> l:st #st_a #st_b #o_a #o_b #m -> a:st -> b:st -> o1:op -> o2:op -> ob:op -> ol:op ->
+  Lemma (requires (Fst_then_snd? (rc #st_a #st_b #o_a #o_b #m o2 o1) \/ Either? (rc #st_a #st_b #o_a #o_b #m o2 o1)) /\ get_rid o1 <> get_rid o2 /\ Fst_then_snd? (rc #st_a #st_b #o_a #o_b #m ob ol) /\ get_rid ob <> get_rid ol /\
+                    distinct_ops o1 o2 /\ distinct_ops o1 ob /\ distinct_ops o1 ol /\ distinct_ops o2 ob /\ distinct_ops o2 ol /\ distinct_ops ob ol /\
+                    eq (merge (do l ol) (do (do a ol) o1) (do (do b ol) o2)) (do (merge (do l ol) (do a ol) (do (do b ol) o2)) o1))
+          (ensures eq (merge (do l ol) (do (do (do a ob) ol) o1) (do (do b ol) o2)) (do (merge (do l ol) (do (do a ob) ol) (do (do b ol) o2)) o1))
+          
+let inter_left_base_2op #st_a #st_b #o_a #o_b #m #v l a b o1 o2 ob ol =
+  let k = get_key ol in
+  let ka = Alpha_t k in let kb = Beta_t k in
+  if get_key o1 = k && get_key o2 = k && get_key ob = k && is_alpha_op o1 && is_alpha_op o2 && is_alpha_op ob && is_alpha_op ol && (Fst_then_snd? (m.rc_a (get_op_a o2) (get_op_a o1)) || Either? (m.rc_a (get_op_a o2) (get_op_a o1))) && Fst_then_snd? (m.rc_a (get_op_a ob) (get_op_a ol)) then
+      v.inter_left_base_2op_a (sel l ka) (sel a ka) (sel b ka) (get_op_a o1) (get_op_a o2) (get_op_a ob) (get_op_a ol)
+  else if get_key o1 = k && get_key o2 = k && get_key ob = k && is_beta_op o1 && is_beta_op o2 && is_beta_op ob && is_beta_op ol && (Fst_then_snd? (m.rc_b (get_op_b o2) (get_op_b o1)) || Either? (m.rc_b (get_op_b o2) (get_op_b o1))) && Fst_then_snd? (m.rc_b (get_op_b ob) (get_op_b ol)) then
+      v.inter_left_base_2op_b (sel l kb) (sel a kb) (sel b kb) (get_op_b o1) (get_op_b o2) (get_op_b ob) (get_op_b ol)
+  else if Either? (rc #st_a #st_b #o_a #o_b #m o2 o1) then v.inter_left_base_2op' l a b o1 o2 ob ol
+  else ()
+
+val inter_right_2op : #st_a:Type0 -> #st_b:Type0 -> #o_a:eqtype -> #o_b:eqtype -> #m:(json st_a st_b o_a o_b) -> #v:(vc st_a st_b o_a o_b m) -> l:st #st_a #st_b #o_a #o_b #m -> a:st -> b:st -> o1:op -> o2:op -> ob:op -> ol:op -> o:op ->
+  Lemma (requires (Fst_then_snd? (rc #st_a #st_b #o_a #o_b #m o2 o1) \/ Either? (rc #st_a #st_b #o_a #o_b #m o2 o1)) /\ get_rid o1 <> get_rid o2 /\ Fst_then_snd? (rc #st_a #st_b #o_a #o_b #m ob ol) /\ get_rid ob <> get_rid ol /\
+                    (~ (Either? (rc #st_a #st_b #o_a #o_b #m o ob)) \/ Fst_then_snd? (rc #st_a #st_b #o_a #o_b #m o ol)) /\               
+                    distinct_ops o1 o2 /\ distinct_ops o1 ob /\ distinct_ops o1 ol /\ distinct_ops o1 o /\ distinct_ops o2 ob /\ distinct_ops o2 ol /\ distinct_ops o2 o /\ distinct_ops ob ol /\ distinct_ops ob o /\ distinct_ops ol o /\
+                    get_rid o <> get_rid ol /\ //from app.fsti
+                    eq (merge (do l ol) (do (do a ol) o1) (do (do (do b ob) ol) o2)) (do (merge (do l ol) (do a ol) (do (do (do b ob) ol) o2)) o1))
+          (ensures eq (merge (do l ol) (do (do a ol) o1) (do (do (do (do b o) ob) ol) o2)) (do (merge (do l ol) (do a ol) (do (do (do (do b o) ob) ol) o2)) o1))
+          
+let inter_right_2op #st_a #st_b #o_a #o_b #m #v l a b o1 o2 ob ol o =
+  let k = get_key o in
+  let ka = Alpha_t k in let kb = Beta_t k in
+  if get_key o1 = k && get_key o2 = k && get_key ob = k && get_key ol = k && is_alpha_op o1 && is_alpha_op o2 && is_alpha_op ob && is_alpha_op ol && is_alpha_op o && (Fst_then_snd? (m.rc_a (get_op_a o2) (get_op_a o1)) || Either? (m.rc_a (get_op_a o2) (get_op_a o1))) && Fst_then_snd? (m.rc_a (get_op_a ob) (get_op_a ol)) && (Fst_then_snd? (m.rc_a (get_op_a o) (get_op_a ob)) || Snd_then_fst? (m.rc_a (get_op_a o) (get_op_a ob)) || Fst_then_snd? (m.rc_a (get_op_a o) (get_op_a ol))) then 
+    v.inter_right_2op_a (sel l ka) (sel a ka) (sel b ka) (get_op_a o1) (get_op_a o2) (get_op_a ob) (get_op_a ol) (get_op_a o)
+  else if get_key o1 = k && get_key o2 = k && get_key ob = k && get_key ol = k && is_beta_op o1 && is_beta_op o2 && is_beta_op ob && is_beta_op ol && is_beta_op o && (Fst_then_snd? (m.rc_b (get_op_b o2) (get_op_b o1)) || Either? (m.rc_b (get_op_b o2) (get_op_b o1))) && Fst_then_snd? (m.rc_b (get_op_b ob) (get_op_b ol)) && (Fst_then_snd? (m.rc_b (get_op_b o) (get_op_b ob)) || Snd_then_fst? (m.rc_b (get_op_b o) (get_op_b ob)) || Fst_then_snd? (m.rc_b (get_op_b o) (get_op_b ol))) then
+    v.inter_right_2op_b (sel l kb) (sel a kb) (sel b kb) (get_op_b o1) (get_op_b o2) (get_op_b ob) (get_op_b ol) (get_op_b o)
+  else if Either? (rc #st_a #st_b #o_a #o_b #m o2 o1) then v.inter_right_2op' l a b o1 o2 ob ol o
+  else ()
+
+val inter_left_2op : #st_a:Type0 -> #st_b:Type0 -> #o_a:eqtype -> #o_b:eqtype -> #m:(json st_a st_b o_a o_b) -> #v:(vc st_a st_b o_a o_b m) -> l:st #st_a #st_b #o_a #o_b #m -> a:st -> b:st -> o1:op -> o2:op -> ob:op -> ol:op -> o:op ->
+  Lemma (requires (Fst_then_snd? (rc #st_a #st_b #o_a #o_b #m o2 o1) \/ Either? (rc #st_a #st_b #o_a #o_b #m o2 o1)) /\ get_rid o1 <> get_rid o2 /\ Fst_then_snd? (rc #st_a #st_b #o_a #o_b #m ob ol) /\ get_rid ob <> get_rid ol /\
+                    (~ (Either? (rc #st_a #st_b #o_a #o_b #m o ob)) \/ Fst_then_snd? (rc #st_a #st_b #o_a #o_b #m o ol)) /\               
+                    distinct_ops o1 o2 /\ distinct_ops o1 ob /\ distinct_ops o1 ol /\ distinct_ops o1 o /\ distinct_ops o2 ob /\ distinct_ops o2 ol /\ distinct_ops o2 o /\ distinct_ops ob ol /\ distinct_ops ob o /\ distinct_ops ol o /\
+                    get_rid o <> get_rid ol /\ //from app.fsti
+                    eq (merge (do l ol) (do (do a ol) o1) (do (do (do b ob) ol) o2)) (do (merge (do l ol) (do a ol) (do (do (do b ob) ol) o2)) o1))
+          (ensures eq (merge (do l ol) (do (do (do a o) ol) o1) (do (do (do b ob) ol) o2)) (do (merge (do l ol) (do (do a o) ol) (do (do (do b ob) ol) o2)) o1)) 
+
+let inter_left_2op #st_a #st_b #o_a #o_b #m #v l a b o1 o2 ob ol o =
+  let k = get_key o in
+  let ka = Alpha_t k in let kb = Beta_t k in
+  if get_key o1 = k && get_key o2 = k && get_key ob = k && get_key ol = k && is_alpha_op o1 && is_alpha_op o2 && is_alpha_op ob && is_alpha_op ol && is_alpha_op o && (Fst_then_snd? (m.rc_a (get_op_a o2) (get_op_a o1)) || Either? (m.rc_a (get_op_a o2) (get_op_a o1))) && Fst_then_snd? (m.rc_a (get_op_a ob) (get_op_a ol)) && (Fst_then_snd? (m.rc_a (get_op_a o) (get_op_a ob)) || Snd_then_fst? (m.rc_a (get_op_a o) (get_op_a ob)) || Fst_then_snd? (m.rc_a (get_op_a o) (get_op_a ol))) then 
+    v.inter_left_2op_a (sel l ka) (sel a ka) (sel b ka) (get_op_a o1) (get_op_a o2) (get_op_a ob) (get_op_a ol) (get_op_a o)
+  else if get_key o1 = k && get_key o2 = k && get_key ob = k && get_key ol = k && is_beta_op o1 && is_beta_op o2 && is_beta_op ob && is_beta_op ol && is_beta_op o && (Fst_then_snd? (m.rc_b (get_op_b o2) (get_op_b o1)) || Either? (m.rc_b (get_op_b o2) (get_op_b o1))) && Fst_then_snd? (m.rc_b (get_op_b ob) (get_op_b ol)) && (Fst_then_snd? (m.rc_b (get_op_b o) (get_op_b ob)) || Snd_then_fst? (m.rc_b (get_op_b o) (get_op_b ob)) || Fst_then_snd? (m.rc_b (get_op_b o) (get_op_b ol))) then
+    v.inter_left_2op_b (sel l kb) (sel a kb) (sel b kb) (get_op_b o1) (get_op_b o2) (get_op_b ob) (get_op_b ol) (get_op_b o)
+  else if Either? (rc #st_a #st_b #o_a #o_b #m o2 o1) then v.inter_left_2op' l a b o1 o2 ob ol o
+  else ()
+
 val ind_right_2op : #st_a:Type0 -> #st_b:Type0 -> #o_a:eqtype -> #o_b:eqtype -> #m:(json st_a st_b o_a o_b) -> #v:(vc st_a st_b o_a o_b m) -> l:st #st_a #st_b #o_a #o_b #m -> a:st #st_a #st_b #o_a #o_b #m -> b:st #st_a #st_b #o_a #o_b #m -> o1:op -> o2:op -> o2':op -> 
   Lemma (requires Fst_then_snd? (rc #st_a #st_b #o_a #o_b #m o2 o1) /\ get_rid o1 <> get_rid o2 /\
                     distinct_ops o1 o2 /\ distinct_ops o1 o2' /\ distinct_ops o2 o2' /\
@@ -294,163 +514,18 @@ let ind_right_2op #st_a #st_b #o_a #o_b #m #v l a b o1 o2 o2' =
   else if get_key o1 = k && get_key o2 = k && is_beta_op o1 && is_beta_op o2 && is_beta_op o2' && Fst_then_snd? (m.rc_b (get_op_b o2) (get_op_b o1)) then
       v.ind_right_2op_b (sel l kb) (sel a kb) (sel b kb) (get_op_b o1) (get_op_b o2) (get_op_b o2')
   else ()
-  
-(*class vc (st:Type0) (app_op:eqtype) (m:mrdt st app_op) = {
-  merge_comm : l:st -> a:st -> b:st ->
-    Lemma (ensures (m.eq (m.merge l a b) (m.merge l b a)));
 
-  merge_idem : s:st ->
-    Lemma (ensures (m.eq (m.merge s s s) s));
+val ind_left_2op : #st_a:Type0 -> #st_b:Type0 -> #o_a:eqtype -> #o_b:eqtype -> #m:(json st_a st_b o_a o_b) -> #v:(vc st_a st_b o_a o_b m) -> l:st #st_a #st_b #o_a #o_b #m -> a:st #st_a #st_b #o_a #o_b #m -> b:st #st_a #st_b #o_a #o_b #m -> o1:op -> o2:op -> o1':op -> 
+  Lemma (requires Fst_then_snd? (rc #st_a #st_b #o_a #o_b #m o2 o1) /\ get_rid o1 <> get_rid o2 /\
+                    distinct_ops o1 o2 /\ distinct_ops o1 o1' /\ distinct_ops o2 o1' /\
+                    eq (merge l (do a o1) (do b o2)) (do (merge l a (do b o2)) o1))
+          (ensures eq (merge l (do (do a o1') o1) (do b o2)) (do (merge l (do a o1') (do b o2)) o1))
 
-  base_2op : o1:op -> o2:op ->
-    Lemma (requires (Fst_then_snd? (m.rc o2 o1) \/ Either? (m.rc o2 o1)) /\ get_rid o1 <> get_rid o2 /\ distinct_ops o1 o2)
-          (ensures m.eq (m.merge m.init_st (m.do m.init_st o1) (m.do m.init_st o2)) (m.do (m.merge m.init_st m.init_st (m.do m.init_st o2)) o1));
-
-  ind_lca_2op : l:st -> o1:op -> o2:op -> ol:op ->
-  Lemma (requires (Fst_then_snd? (m.rc o2 o1) \/ Either? (m.rc o2 o1)) /\
-                  get_rid o1 <> get_rid o2 /\
-                  distinct_ops o1 o2 /\
-                  distinct_ops o1 ol /\
-                  distinct_ops o2 ol /\
-                  m.eq (m.merge l (m.do l o1) (m.do l o2)) (m.do (m.merge l l (m.do l o2)) o1))
-        (ensures m.eq (m.merge (m.do l ol) (m.do (m.do l ol) o1) (m.do (m.do l ol) o2)) (m.do (m.merge (m.do l ol) (m.do l ol) (m.do (m.do l ol) o2)) o1));
-
-  inter_right_base_2op : l:st -> a:st -> b:st -> o1:op -> o2:op -> ob:op -> ol:op ->
-  Lemma (requires (Fst_then_snd? (m.rc o2 o1) \/ Either? (m.rc o2 o1)) /\
-                  get_rid o1 <> get_rid o2 /\
-                  Fst_then_snd? (m.rc ob ol) /\
-                  get_rid ob <> get_rid ol /\
-                  distinct_ops o1 o2 /\
-                  distinct_ops o1 ob /\
-                  distinct_ops o1 ol /\
-                  distinct_ops o2 ob /\
-                  distinct_ops o2 ol /\
-                  distinct_ops ob ol /\
-                  m.eq (m.merge l (m.do a o1) (m.do b o2)) (m.do (m.merge l a (m.do b o2)) o1) /\
-                  m.eq (m.merge l (m.do a o1) (m.do (m.do b ob) o2)) (m.do (m.merge l a (m.do (m.do b ob) o2)) o1) /\
-                  m.eq (m.merge (m.do l ol) (m.do (m.do a ol) o1) (m.do (m.do b ol) o2)) (m.do (m.merge (m.do l ol) (m.do a ol) (m.do (m.do b ol) o2)) o1))
-        (ensures m.eq (m.merge (m.do l ol) (m.do (m.do a ol) o1) (m.do (m.do (m.do b ob) ol) o2)) (m.do (m.merge (m.do l ol) (m.do a ol) (m.do (m.do (m.do b ob) ol) o2)) o1));
-
-inter_left_base_2op : l:st -> a:st -> b:st -> o1:op -> o2:op -> ob:op -> ol:op ->
-  Lemma (requires Fst_then_snd? (m.rc o2 o1) /\
-                  Fst_then_snd? (m.rc ob ol) /\
-                  get_rid o2 <> get_rid o1 /\
-                  get_rid ob <> get_rid ol /\
-                  distinct_ops o1 o2 /\
-                  distinct_ops o1 ob /\
-                  distinct_ops o1 ol /\
-                  distinct_ops o2 ob /\
-                  distinct_ops o2 ol /\
-                  distinct_ops ob ol /\
-                  m.eq (m.merge (m.do l ol) (m.do (m.do a ol) o1) (m.do (m.do b ol) o2)) (m.do (m.merge (m.do l ol) (m.do a ol) (m.do (m.do b ol) o2)) o1))
-        (ensures m.eq (m.merge (m.do l ol) (m.do (m.do (m.do a ob) ol) o1) (m.do (m.do b ol) o2)) (m.do (m.merge (m.do l ol) (m.do (m.do a ob) ol) (m.do (m.do b ol) o2)) o1));
-
-inter_right_2op : l:st -> a:st -> b:st -> o1:op -> o2:op -> ob:op -> ol:op -> o:op ->
-  Lemma (requires (Fst_then_snd? (m.rc o2 o1) \/ Either? (m.rc o2 o1)) /\
-                  get_rid o1 <> get_rid o2 /\
-                  Fst_then_snd? (m.rc ob ol) /\
-                  get_rid ob <> get_rid ol /\
-                  (~ (Either? (m.rc o ob)) \/ Fst_then_snd? (m.rc o ol)) /\
-                  distinct_ops o1 o2 /\
-                  distinct_ops o1 ob /\
-                  distinct_ops o1 ol /\
-                  distinct_ops o1 o /\
-                  distinct_ops o2 ob /\
-                  distinct_ops o2 ol /\
-                  distinct_ops o2 o /\
-                  distinct_ops ob ol /\
-                  distinct_ops ob o /\
-                  distinct_ops ol o /\
-                  get_rid o <> get_rid ol /\
-                  m.eq (m.merge (m.do l ol) (m.do (m.do a ol) o1) (m.do (m.do (m.do b ob) ol) o2)) (m.do (m.merge (m.do l ol) (m.do a ol) (m.do (m.do (m.do b ob) ol) o2)) o1))
-        (ensures m.eq (m.merge (m.do l ol) (m.do (m.do a ol) o1) (m.do (m.do (m.do (m.do b o) ob) ol) o2)) (m.do (m.merge (m.do l ol) (m.do a ol) (m.do (m.do (m.do (m.do b o) ob) ol) o2)) o1));
-
-inter_left_2op : l:st -> a:st -> b:st -> o1:op -> o2:op -> ob:op -> ol:op -> o:op ->
-  Lemma (requires Fst_then_snd? (m.rc o2 o1) /\
-                  Fst_then_snd? (m.rc ob ol) /\
-                  get_rid o2 <> get_rid o1 /\
-                  get_rid ob <> get_rid ol /\
-                  (~ (Either? (m.rc o ob)) \/ Fst_then_snd? (m.rc o ol)) /\
-                  distinct_ops o1 o2 /\
-                  distinct_ops o1 ob /\
-                  distinct_ops o1 ol /\
-                  distinct_ops o1 o /\
-                  distinct_ops o2 ob /\
-                  distinct_ops o2 ol /\
-                  distinct_ops o2 o /\
-                  distinct_ops ob ol /\
-                  distinct_ops ob o /\
-                  distinct_ops ol o /\
-                  get_rid o <> get_rid ol /\
-                  m.eq (m.merge (m.do l ol) (m.do (m.do a ol) o1) (m.do (m.do (m.do b ob) ol) o2)) (m.do (m.merge (m.do l ol) (m.do a ol) (m.do (m.do (m.do b ob) ol) o2)) o1))
-        (ensures m.eq (m.merge (m.do l ol) (m.do (m.do (m.do a o) ol) o1) (m.do (m.do (m.do b ob) ol) o2)) (m.do (m.merge (m.do l ol) (m.do (m.do a o) ol) (m.do (m.do (m.do b ob) ol) o2)) o1));
-
-ind_right_2op : l:st -> a:st -> b:st -> o1:op -> o2:op -> o2':op ->
-  Lemma (requires Fst_then_snd? (m.rc o2 o1) /\
-                  get_rid o1 <> get_rid o2 /\
-                  distinct_ops o1 o2 /\
-                  distinct_ops o1 o2' /\
-                  distinct_ops o2 o2' /\
-                  m.eq (m.merge l (m.do a o1) (m.do b o2)) (m.do (m.merge l a (m.do b o2)) o1))
-        (ensures m.eq (m.merge l (m.do a o1) (m.do (m.do b o2') o2)) (m.do (m.merge l a (m.do (m.do b o2') o2)) o1));
-
-ind_left_2op : l:st -> a:st -> b:st -> o1:op -> o2:op -> o1':op ->
-  Lemma (requires (Fst_then_snd? (m.rc o2 o1) \/ Either? (m.rc o2 o1)) /\
-                  get_rid o1 <> get_rid o2 /\
-                  distinct_ops o1 o2 /\
-                  distinct_ops o1 o1' /\
-                  distinct_ops o2 o1' /\
-                  m.eq (m.merge l (m.do a o1) (m.do b o2)) (m.do (m.merge l a (m.do b o2)) o1))
-        (ensures m.eq (m.merge l (m.do (m.do a o1') o1) (m.do b o2)) (m.do (m.merge l (m.do a o1') (m.do b o2)) o1));
-
-  base_1op : o1:op ->
-  Lemma (ensures m.eq (m.merge m.init_st (m.do m.init_st o1) m.init_st) (m.do (m.merge m.init_st m.init_st m.init_st) o1));
-
-ind_lca_1op : l:st -> o1:op -> ol:op ->
-  Lemma (requires distinct_ops o1 ol /\
-                  m.eq (m.merge l (m.do l o1) l) (m.do (m.merge l l l) o1))
-        (ensures m.eq (m.merge (m.do l ol) (m.do (m.do l ol) o1) (m.do l ol)) (m.do (m.merge (m.do l ol) (m.do l ol) (m.do l ol)) o1));
-
-inter_right_base_1op : l:st -> a:st -> b:st -> o1:op -> ob:op -> ol:op ->
-  Lemma (requires Fst_then_snd? (m.rc ob ol) /\ get_rid ob <> get_rid ol /\
-                    distinct_ops o1 ob /\ distinct_ops o1 ol /\ distinct_ops ob ol /\
-                    (Fst_then_snd? (m.rc ob o1) ==> m.eq (m.merge l (m.do a o1) (m.do b ob)) (m.do (m.merge l a (m.do b ob)) o1)) /\
-                    m.eq (m.merge (m.do l ol) (m.do (m.do a ol) o1) (m.do b ol)) (m.do (m.merge (m.do l ol) (m.do a ol) (m.do b ol)) o1))
-          (ensures m.eq (m.merge (m.do l ol) (m.do (m.do a ol) o1) (m.do (m.do b ob) ol)) (m.do (m.merge (m.do l ol) (m.do a ol) (m.do (m.do b ob) ol)) o1));
-
-inter_left_base_1op : l:st -> a:st -> b:st -> o1:op -> ob:op -> ol:op ->
-  Lemma (requires Fst_then_snd? (m.rc ob ol) /\ get_rid ob <> get_rid ol /\
-                    distinct_ops o1 ob /\ distinct_ops o1 ol /\ distinct_ops ob ol /\
-                    m.eq (m.merge (m.do l ol) (m.do (m.do a ol) o1) (m.do b ol)) (m.do (m.merge (m.do l ol) (m.do a ol) (m.do b ol)) o1))
-          (ensures m.eq (m.merge (m.do l ol) (m.do (m.do (m.do a ob) ol) o1) (m.do b ol)) (m.do (m.merge (m.do l ol) (m.do (m.do a ob) ol) (m.do b ol)) o1));
-          
-inter_right_1op : l:st -> a:st -> b:st -> o1:op -> ob:op -> ol:op -> o:op ->
-  Lemma (requires Fst_then_snd? (m.rc ob ol) /\ get_rid ob <> get_rid ol /\
-                    (~ (Either? (m.rc o ob)) \/ Fst_then_snd? (m.rc o ol)) /\
-                    distinct_ops o1 ob /\ distinct_ops o1 ol /\ distinct_ops o1 o /\ distinct_ops ob ol /\ distinct_ops ob o /\ distinct_ops ol o /\
-                    get_rid o <> get_rid ol /\
-                    m.eq (m.merge (m.do l ol) (m.do (m.do a ol) o1) (m.do (m.do b ob) ol)) (m.do (m.merge (m.do l ol) (m.do a ol) (m.do (m.do b ob) ol)) o1))
-          (ensures m.eq (m.merge (m.do l ol) (m.do (m.do a ol) o1) (m.do (m.do (m.do b o) ob) ol)) (m.do (m.merge (m.do l ol) (m.do a ol) (m.do (m.do (m.do b o) ob) ol)) o1));
-
-inter_left_1op : l:st -> a:st -> b:st -> o1:op -> ob:op -> ol:op -> o:op ->
-  Lemma (requires Fst_then_snd? (m.rc ob ol) /\ get_rid ob <> get_rid ol /\
-                    (~ (Either? (m.rc o ob)) \/ Fst_then_snd? (m.rc o ol)) /\
-                    distinct_ops o1 ob /\ distinct_ops o1 ol /\ distinct_ops o1 o /\ distinct_ops ob ol /\ distinct_ops ob o /\ distinct_ops ol o /\
-                    get_rid o <> get_rid ol /\
-                    m.eq (m.merge (m.do l ol) (m.do (m.do (m.do a ob) ol) o1) (m.do b ol)) (m.do (m.merge (m.do l ol) (m.do (m.do a ob) ol) (m.do b ol)) o1))
-          (ensures m.eq (m.merge (m.do l ol) (m.do (m.do (m.do (m.do a o) ob) ol) o1) (m.do b ol)) (m.do (m.merge (m.do l ol) (m.do (m.do (m.do a o) ob) ol) (m.do b ol)) o1));
-
-ind_left_1op : l:st -> a:st -> b:st -> o1:op -> o1':op -> ol:op ->
-  Lemma (requires distinct_ops o1 o1' /\ distinct_ops o1 ol /\ distinct_ops o1' ol /\
-                    m.eq (m.merge (m.do l ol) (m.do a o1) (m.do b ol)) (m.do (m.merge (m.do l ol) a (m.do b ol)) o1))
-          (ensures m.eq (m.merge (m.do l ol) (m.do (m.do a o1') o1) (m.do b ol)) (m.do (m.merge (m.do l ol) (m.do a o1') (m.do b ol)) o1));
-
-ind_right_1op : l:st -> a:st -> b:st -> o2:op -> o2':op -> ol:op ->
-  Lemma (requires distinct_ops o2 o2' /\ distinct_ops o2 ol /\ distinct_ops o2' ol /\
-                    m.eq (m.merge (m.do l ol) (m.do a ol) (m.do b o2)) (m.do (m.merge (m.do l ol) (m.do a ol) b) o2))
-          (ensures m.eq (m.merge (m.do l ol) (m.do a ol) (m.do (m.do b o2') o2)) (m.do (m.merge (m.do l ol) (m.do a ol) (m.do b o2')) o2));
-
-lem_0op : l:st -> a:st -> b:st -> ol:op ->
-  Lemma (ensures m.eq (m.merge (m.do l ol) (m.do a ol) (m.do b ol)) (m.do (m.merge l a b) ol))
-}
-*)
+let ind_left_2op #st_a #st_b #o_a #o_b #m #v l a b o1 o2 o1' =
+  let k = get_key o1' in
+  let ka = Alpha_t k in let kb = Beta_t k in
+  if get_key o1 = k && get_key o2 = k && is_alpha_op o1 && is_alpha_op o2 && is_alpha_op o1' && Fst_then_snd? (m.rc_a (get_op_a o2) (get_op_a o1)) then
+      v.ind_left_2op_a (sel l ka) (sel a ka) (sel b ka) (get_op_a o1) (get_op_a o2) (get_op_a o1')
+  else if get_key o1 = k && get_key o2 = k && is_beta_op o1 && is_beta_op o2 && is_beta_op o1' && Fst_then_snd? (m.rc_b (get_op_b o2) (get_op_b o1)) then
+      v.ind_left_2op_b (sel l kb) (sel a kb) (sel b kb) (get_op_b o1) (get_op_b o2) (get_op_b o1')
+  else ()
