typeclass/Ctr_set.fst
@@ -15,6 +15,13 @@ let cond_comm_base s o1 o2 o3 = ()
 let cond_comm_ind s o1 o2 o3 o l = ()
 
 let base_2op' o1 o2 t = ()
+let ind_lca_2op' l o1 o2 ol = ()
+let inter_right_base_2op' l a b o1 o2 ob ol = ()
+let inter_left_base_2op' l a b o1 o2 ob ol = ()
+let inter_right_2op' l a b o1 o2 ob ol o = ()
+let inter_left_2op' l a b o1 o2 ob ol o = ()
+let ind_right_2op' l a b o1 o2 o2' = ()
+let ind_left_2op' l a b o1 o2 o1' = ()
 
 #set-options "--z3rlimit 100 --ifuel 3"
 instance ictr_set : json C.st S.st C.app_op S.app_op = {
@@ -22,14 +29,15 @@ instance ictr_set : json C.st S.st C.app_op S.app_op = {
   Json1.init_st_b = S.init_st;
   Json1.eq_a = C.eq;
   Json1.eq_b = S.eq;
-  Json1.lem_eq_a;
-  Json1.lem_eq_b;
   Json1.rc_a = C.rc;
   Json1.rc_b = S.rc;
   Json1.do_a = C.do;
   Json1.do_b = S.do;
   Json1.merge_a = C.merge;
-  Json1.merge_b = S.merge
+  Json1.merge_b = S.merge;
+
+  Json1.lem_eq_a;
+  Json1.lem_eq_b;
 }
 
 instance ictr_set_cond : cond C.st S.st C.app_op S.app_op ictr_set = {
@@ -46,5 +54,33 @@ instance ictr_set_proof : vc C.st S.st C.app_op S.app_op ictr_set = {
   Json1.merge_idem_b = S.merge_idem;
   Json1.base_2op_a = C.base_2op;
   Json1.base_2op_b = S.base_2op;
+  Json1.ind_lca_2op_a = C.ind_lca_2op;
+  Json1.ind_lca_2op_b = S.ind_lca_2op;
+  Json1.inter_right_base_2op_a = C.inter_right_base_2op;
+  Json1.inter_right_base_2op_b = S.inter_right_base_2op;
+  Json1.inter_left_base_2op_a = C.inter_left_base_2op;
+  Json1.inter_left_base_2op_b = S.inter_left_base_2op;
+  Json1.inter_right_2op_a = C.inter_right_2op;
+  Json1.inter_right_2op_b = S.inter_right_2op;
+  Json1.inter_left_2op_a = C.inter_left_2op;
+  Json1.inter_left_2op_b = S.inter_left_2op;
+  Json1.ind_right_2op_a = C.ind_right_2op;
+  Json1.ind_right_2op_b = S.ind_right_2op;
+  Json1.ind_left_2op_a = C.ind_left_2op;
+  Json1.ind_left_2op_b = S.ind_left_2op;
+  
   Json1.base_2op';
+  Json1.ind_lca_2op';
+  Json1.inter_right_base_2op';
+  Json1.inter_left_base_2op';
+  Json1.inter_right_2op'; 
+  Json1.inter_left_2op';
+}
+ 
+instance json #st_a #st_b #o_a #o_b #m: L.mrdt st app_op = {
+  Library.init_st = admit();
+  Library.eq;
+  Library.rc = rc #st_a #st_b #o_a #o_b #m;
+  Library.do;
+  Library.merge = merge #st_a #st_b #o_a #o_b #m
 }
